Q4: 1

Q4.dfy
@@ -1,4 +1,4 @@
-Question 4: Factorial
+//Question 4: Factorial
 
 method ComputeFact(n : nat) returns (res : nat)
   requires n > 0;
@@ -13,13 +13,37 @@ method ComputeFact(n : nat) returns (res : nat)
   }
  }
  
- The variables are natural numbers. You are supposed to prove that the program is correct with respect to a recursive definition 
+ /*The variables are natural numbers. You are supposed to prove that the program is correct with respect to a recursive definition
   of the factorial function, defined mathematically as:
   
   fact(1) = 1
   fact(m) = m * fact(m - 1)
-
- 
  
  1.Complete the specification so that Dafny is able to prove ComputeFact correct.
+    method ComputeFact(n : nat) returns (res : nat)
+      requires n > 0;
+      ensures res == fact(n);
+     {
+      res := 1;
+      var i := 2;
+      while (i <= n)
+        invariant 2 <= i <= n + 1;
+        invariant res == fact(i - 1);
+        decreases(n - i);
+      {
+        res := res * i;
+        i := i + 1;
+      }
+     }
+
+     function fact(n : int) : int
+     requires 0 <= n;
+     {
+         if n == 0 then 1 else n * fact(n - 1)
+    }
+
  2.Prove correctness of the loop using the checklist for proving loops correct from the lecture notes. See also Chapter 11 of [Gries].
+
+
+
+*/
